\documentclass{scrartcl}

\begin{document}
	
\begin{equation}
	y_0 = (x_0 \wedge x_1) \wedge (( \lnot x_2 \wedge x_3) \lor (x_2 \wedge  \lnot x_3) \lor (x_2 \wedge x_3) \lor ( \lnot x_2 \wedge  \lnot x_3))
\end{equation}

\begin{equation}
	y_1 = (x_0 \wedge x_1) \wedge (( \lnot x_2 \wedge x_3) \lor (x_2 \wedge  \lnot x_3) \lor (x_2 \wedge x_3))
\end{equation}

\begin{equation}
	y_2 = (x_0 \wedge x_1) \wedge (( \lnot x_2 \wedge x_3) \lor (x_2 \wedge  \lnot x_3) \lor (x_2 \wedge x_3))
\end{equation}

\begin{equation}
	y_3 = (x_0 \wedge x_3 \wedge x_1) \wedge ( \lnot x_2 \lor x_2)
\end{equation}

\end{document}
