\documentclass{scrartcl}

\begin{document}
	
$$y_0 = ( \lnot x_0 \wedge  \lnot x_1 \wedge  \lnot x_2) \lor (x_0 \wedge  \lnot x_1 \wedge  \lnot x_2) \lor (x_0 \wedge  \lnot x_1 \wedge x_2)$$

$$y_1 = ( \lnot x_0 \wedge  \lnot x_1 \wedge  \lnot x_2) \lor ( \lnot x_0 \wedge  \lnot x_1 \wedge x_2) \lor (x_0 \wedge x_1 \wedge x_2) \lor (x_0 \wedge  \lnot x_1 \wedge x_2)$$

$$y_2 = ( \lnot x_0 \wedge  \lnot x_1 \wedge  \lnot x_2) \lor ( \lnot x_0 \wedge  \lnot x_1 \wedge x_2) \lor (x_0 \wedge x_1 \wedge x_2)$$

\end{document}
